Working on aesgctr finally

src/crypto/aes/testgcm.c
@@ -1,0 +1,14 @@
+/* Test code for AES GCM. 
+   Brian Milnes, 14 Aug 2017.
+*/
+#include <stdlib.h>
+#include <stdio.h>
+#include <stdint.h> // for uint?_t
+#include <string.h> // for memcmp
+#include "gcc_compat.h"
+
+int __cdecl main(void) {
+  printf("AES128 GCM tests\n");
+  printf("Nothing implemented.\n");
+  printf("\nAES128 GCM tests completed.");
+}
