src/crypto/aes/aes-x64/ctr_helpers.i.dfy
@@ -371,5 +371,21 @@ lemma {:timeLimitMultiplier 3} lemma_CTR_Encrypt_Upto_Done(g : G, iv : uint64, i
   lemma_CTR_Encrypt_length'(g.inp, g.key, g.alg, iv, init_ctr);
 }
 
+lemma lemma_CTROutput(g : G, iv_reg : uint64, init_ctr : uint64, out_ptr : uint64, mem : Heaplets)
+  returns (output : seq<Quadword>)
+  requires CTR_Encrypt_Req(g.inp, g.key, g.alg);
+  requires OutWriteable(g.inp, g.out_heap, out_ptr, mem);
+  requires ValidSrcAddrs(mem, g.out_heap, out_ptr, 128, Secret, SeqLength(g.inp)*16)
+  requires CTR_Encrypt_Upto_Done(g, iv_reg, init_ctr, out_ptr, mem, SeqLength(g.inp));
+  ensures  output == CTR_Encrypt(g.inp, g.key, g.alg, iv_reg, init_ctr);
+{
+  output := CTR_Encrypt(g.inp, g.key, g.alg, iv_reg, init_ctr);
+  lemma_CTR_Encrypt_length(g.inp);
+  assert  forall j : nat :: 0 <= j < |output| ==>
+    output[j] == mem[g.out_heap].quads[out_ptr + j*16].v;
+  assert forall j : nat :: j < |output| ==>
+   CTR_Encrypt(g.inp, g.key, g.alg, iv_reg, init_ctr)[j] == mem[g.out_heap].quads[out_ptr + j * 16].v;
+}
+
 // End of Module
 }
