src/crypto/aes/aes-x64/gcm_helpers.i.dfy
@@ -3,18 +3,24 @@ include "../../../lib/util/operations.s.dfy"
 include "../../../lib/util/words_and_bytes.s.dfy"
 include "../../../lib/collections/Seqs.s.dfy"
 include "../../../arch/x64/vale.i.dfy"
-include "../../../arch/x64/vale64.i.dfy"
 include "../../../lib/util/dafny_wrappers.i.dfy"
-include "../ctr.s.dfy"
-include "../aes.s.dfy"
 
-module proof {
+include "../gcm3.s.dfy"
+
+include "../aes.s.dfy"
+include "../aes_helpers.i.dfy"
+
+module GCMHelpers {
 
 import opened x64_vale_i
 import opened x64_def_s
 import opened types_s
 import opened dafny_wrappers_i
 import opened AESModule
+import opened AESHelpersModule
+import opened GCMModule
+
+
 
 
 }
