src/crypto/loopunroll/copy128.dfy
@@ -1,0 +1,47 @@
+/*
+
+   This is an example of how to specify your input to output mapping and
+ then give it to WritesRegionN each time. Specify the entirety of your 
+ range but then only the number of uint64 written. This makes it easier
+ for Vale to understand the equivalence of values without sequence math. 
+   
+*/
+
+include "../../lib/util/types.s.dfy"
+include "../../arch/x64/def.s.dfy"
+include "../../arch/x64/vale.i.dfy"
+include "regions128.dfy"
+
+module copy128 {
+
+import opened types_s
+import opened x64_def_s
+import opened x64_vale_i
+import opened regions128
+
+function Copy128(mem : Heaplets, id: heaplet_id, base : nat, size: int, i : nat) : Quadword
+ requires 0 <= i < size;
+ requires ValidDstReg128(mem, id, base, size);
+{
+  mem[id].quads[(addr128(base, i))].v
+}
+
+// Generate the whole sequence with this function that knows what the values are to
+// obviate any subsequence proof problems.
+
+function Copy128Seq(mem : Heaplets, id: heaplet_id, base : nat, size : nat, count : nat) : seq<Quadword>
+ requires ValidDstReg128(mem, id, base, size);
+ requires 0 <= count <= size;
+ ensures |Copy128Seq(mem, id, base, size, count)| == count;
+ // Doing this here at the function definition is CRITICAL as it proves and then is available
+ // when you need it in the requirements as
+ ensures forall i : nat :: 0 <= i < count ==>
+         Copy128Seq(mem, id, base, size, count)[i] == Copy128(mem, id, base, size, i);
+{
+  if (count == 0) then
+    []
+  else 
+    Copy128Seq(mem, id, base, size, count - 1) + [Copy128(mem, id, base, size, count - 1)]
+}
+
+}
